Hoare/Logic.thy
@@ -62,7 +62,7 @@ proof
   obtain st' where St' : "evalYulStep D st = YulResult st'"  and Q : "Q st'"
     using H[OF P] by auto
 
-  hence "evalYul' D st 1 = YulResult st'" by auto
+  hence "evalYul' D st 1 = YulResult st'" by(auto split:YulMode.splits)
 
   thus "\<exists>n st' . evalYul' D st n = YulResult st' \<and>  Q st'" using St' Q by blast
 qed
@@ -136,122 +136,837 @@ break and continue will add a (possibly empty) prefix to the stack, and drop the
 delta function that precisely describes the
 change to the continuation *)
 
-lemma evalYulStep_cont_pref :
+lemma evalYulStep_cont_prefix_reg :
   assumes Hcont : "cont st = h#t"
   assumes Hstep : "evalYulStep D st = YulResult st'"
   shows "\<exists> pre . cont st' = pre @ t" 
-proof(cases h)
-  case (EnterStatement st)
+proof(cases "mode st")
+  case Regular
   show ?thesis
-  proof(cases st)
-    case (YulFunctionCallStatement x)
-    then show ?thesis using assms EnterStatement
-      by(cases x; auto)
+  proof(cases h)
+    case (EnterStatement st)
+    then show ?thesis using assms Regular
+      by(auto simp add: updateResult_def split: YulResult.splits option.splits)
   next
-    case (YulAssignmentStatement x)
-    then show ?thesis using assms EnterStatement
-      by(cases x; auto)
+    case (ExitStatement st L F)
+    then show ?thesis using assms Regular
+      by(auto simp add: updateResult_def split: YulResult.splits option.splits)
   next
-    case (YulVariableDeclarationStatement x)
-    show ?thesis
-    proof(cases x)
-      case (YulVariableDeclaration x1 x2)
-      then show ?thesis using assms EnterStatement YulVariableDeclarationStatement 
-        by(cases x2; auto)
-    qed
+    case (EnterFunctionCall name fsig)
+    then show ?thesis using assms Regular
+      by(auto simp add: updateResult_def split: YulResult.splits option.splits)
   next
-    case (YulFunctionDefinitionStatement x)
-    then show ?thesis using assms EnterStatement YulFunctionDefinitionStatement
-      by(auto)
+    case (ExitFunctionCall name vals_old local_old funs_old fsig)
+    then show ?thesis using assms Regular
+      by(auto simp add: updateResult_def split: YulResult.splits option.splits)
   next
-    case (YulIf x1 x2)
-    then show ?thesis using assms EnterStatement by auto
-  next
-    case (YulSwitch x1 x2)
-    then show ?thesis using assms EnterStatement by auto
-  next
-    case (YulForLoop pre cond post body)
-    then show ?thesis using assms EnterStatement 
-      by(cases pre; auto)
-  next
-  case YulBreak
-  then show ?thesis using assms EnterStatement
-    by(auto)
-  next
-    case YulContinue
-    then show ?thesis using assms EnterStatement
-      by auto
-  next
-    case YulLeave
-    then show ?thesis using assms EnterStatement
-      by auto
-  next
-    case (YulBlock x11)
-    then show ?thesis using assms EnterStatement
-      by(auto split: sum.splits)
+    case (Expression e)
+    then show ?thesis using assms Regular
+      by(auto simp add: updateResult_def split: YulResult.splits option.splits)
   qed
 next
-  case (ExitStatement st locals sigs)
-  show ?thesis
-  proof(cases st)
-    case (YulFunctionCallStatement x)
-    then show ?thesis using assms ExitStatement
-      by(cases x; auto split:list.splits)
+  case Break
+  then show ?thesis 
+  proof(cases h)
+    case (EnterStatement st)
+    then show ?thesis using assms Break
+      by(auto simp add: updateResult_def split: YulResult.splits option.splits)
   next
-    case (YulAssignmentStatement x)
-    then show ?thesis using assms ExitStatement
-      by(cases x; auto split:list.splits if_splits option.splits)
+    case (ExitStatement st L F)
+    then show ?thesis using assms Break
+      by(auto split: YulStatement.split_asm)
   next
-    case (YulVariableDeclarationStatement x)
-    show ?thesis
-    proof(cases x)
-      case (YulVariableDeclaration x1 x2)
-      then show ?thesis using assms ExitStatement YulVariableDeclarationStatement 
-        by(cases x2; auto split: if_splits option.splits)
-    qed
+    case (EnterFunctionCall name fsig)
+    then show ?thesis using assms Break
+      by(auto simp add: updateResult_def split: YulResult.splits option.splits)
   next
-    case (YulFunctionDefinitionStatement x) 
-    then show ?thesis using assms ExitStatement YulFunctionDefinitionStatement
+    case (ExitFunctionCall name vals_old local_old funs_old fsig)
+    then show ?thesis using assms Break
+      by(auto simp add: updateResult_def split: YulResult.splits option.splits)
+  next
+    case (Expression e)
+    then show ?thesis using assms Break
+      by(auto simp add: updateResult_def split: YulResult.splits option.splits)
+  qed
+next
+  case Continue
+  then show ?thesis
+  proof(cases h)
+    case (EnterStatement st)
+    then show ?thesis using assms Continue
+      by(auto simp add: updateResult_def split: YulResult.splits option.splits)
+  next
+    case (ExitStatement st L F)
+    then show ?thesis using assms Continue
+      by(auto split: YulStatement.split_asm)
+  next
+    case (EnterFunctionCall name fsig)
+    then show ?thesis using assms Continue
+      by(auto simp add: updateResult_def split: YulResult.splits option.splits)
+  next
+    case (ExitFunctionCall name vals_old local_old funs_old fsig)
+    then show ?thesis using assms Continue
+      by(auto simp add: updateResult_def split: YulResult.splits option.splits)
+  next
+    case (Expression e)
+    then show ?thesis using assms Continue
+      by(auto simp add: updateResult_def split: YulResult.splits option.splits)
+  qed
+next
+  case Leave
+  then show ?thesis 
+  proof(cases h)
+    case (EnterStatement st)
+    then show ?thesis using assms Leave
+      by(auto simp add: updateResult_def split: YulResult.splits option.splits)
+  next
+    case (ExitStatement st L F)
+    then show ?thesis using assms Leave
+      by(auto split: YulStatement.split_asm)
+  next
+    case (EnterFunctionCall name fsig)
+    then show ?thesis using assms Leave
+      by(auto simp add: updateResult_def split: YulResult.splits option.splits)
+  next
+    case (ExitFunctionCall name vals_old local_old funs_old fsig)
+    then show ?thesis using assms Leave
+      by(auto simp add: updateResult_def split: YulResult.splits option.splits)
+  next
+    case (Expression e)
+    then show ?thesis using assms Leave
+      by(auto simp add: updateResult_def split: YulResult.splits option.splits)
+  qed
+qed
+
+lemma evalYul'_step_succeed_prior :
+  assumes H : "evalYul' D input n = YulResult res"
+  assumes "n' \<le> n"
+  shows "\<exists> res' . evalYul' D input n' = YulResult res'" using assms
+proof(induction n arbitrary: D input n' res)
+  case 0
+  then show ?case by auto
+next
+  case (Suc n)
+  show ?case
+  proof(cases "cont input")
+    case Nil
+    then show ?thesis using Suc.prems
       by(auto)
   next
-    case (YulIf x1 x2)
-    then show ?thesis using assms ExitStatement
-      by(auto split:list.splits if_splits)
-  next
-    case (YulSwitch x1 x2)
-    then show ?thesis using assms ExitStatement
-      by(auto split:list.splits if_splits prod.splits option.splits YulSwitchCase.splits YulLiteral.splits)
-  next
-    case (YulForLoop x1 x2 x3 x4)
-    then show ?thesis using assms ExitStatement
-      by(auto split:list.splits if_splits)
-  next
-    case YulBreak
-    then show ?thesis using assms ExitStatement
-      apply(auto split:list.splits if_splits)
-  next
-    case YulContinue
-    then show ?thesis sorry
-  next
-    case YulLeave
-    then show ?thesis sorry
-  next
-    case (YulBlock x11)
-    then show ?thesis sorry
+    case (Cons ch ct)
+
+    show ?thesis using Suc
+    proof(cases "evalYulStep D input")
+      case (ErrorResult x21 x22)
+      then show ?thesis using Suc.prems Cons by auto
+    next
+      case (YulResult res1)
+
+      then have Eval' : "evalYul' D res1 n = YulResult res"
+        using Suc.prems Cons by auto
+
+      have Leq : "n' - 1 \<le> n" using Suc.prems by auto
+
+      obtain penult where Penult :
+        "evalYul' D res1 (n' - 1) = YulResult penult" 
+        using Suc.IH[OF Eval' Leq] by auto
+
+      have FirstStep :
+        "evalYul' D input 1 = YulResult res1"
+        using YulResult
+        by(auto split:YulMode.splits)
+
+      have Conc' : "evalYul' D input (1 + (n' - 1)) = YulResult penult"
+        using evalYul'_steps[OF FirstStep Penult] by auto
+
+      show ?thesis
+      proof(cases n')
+        case Zero' : 0
+        then show ?thesis 
+          by(auto)
+      next
+        case Suc' : (Suc nat)
+
+        hence N'Eq : "(1 + (n' - 1)) = n'"
+          by auto
+
+        show ?thesis using Conc' unfolding N'Eq by blast
+      qed
+    qed
   qed
-    
+qed
+
+lemma evalYulStep_cont_extend :
+  assumes Hstep : "evalYulStep D \<lparr>result = r, cont = h#t\<rparr> = 
+                   YulResult \<lparr>result = r', cont = c'\<rparr>"
+  shows "\<exists> pre . 
+           evalYulStep D \<lparr> result = r, cont = [h] \<rparr> =
+           YulResult \<lparr>result = r', cont = pre \<rparr> \<and>
+           c' = pre @ t" 
+proof(cases "r_mode r")
+  case Regular
+  then show ?thesis
+  proof(cases h)
+    case (EnterStatement st)
+    then show ?thesis using assms Regular
+      by(auto simp add: updateResult_def split: YulResult.splits option.splits)
+  next
+    case (ExitStatement st L F)
+    then show ?thesis using assms Regular
+      by(auto simp add: updateResult_def split: YulResult.splits option.splits)
+  next
+    case (EnterFunctionCall name fsig)
+    then show ?thesis using assms Regular
+      by(auto simp add: updateResult_def split: YulResult.splits option.splits)
+  next
+    case (ExitFunctionCall name vals_old local_old funs_old fsig)
+    then show ?thesis using assms Regular
+      by(auto simp add: updateResult_def split: YulResult.splits option.splits)
+  next
+    case (Expression e)
+    then show ?thesis using assms Regular
+      by(auto simp add: updateResult_def split: YulResult.splits option.splits)
+  qed
 next
-  case (EnterFunctionCall x31 x32)
-  then show ?thesis sorry
+  case Break
+  then show ?thesis  using Hstep
+    by(cases h; auto split: YulStatement.split_asm)
 next
-  case (ExitFunctionCall x41 x42 x43 x44 x45)
-  then show ?thesis sorry
+  case Continue
+  then show ?thesis using Hstep
+    by(cases h; auto split: YulStatement.split_asm)
 next
-  case (Expression x5)
-  then show ?thesis sorry
+  case Leave
+  then show ?thesis using Hstep
+    by(cases h; auto)
 qed
 
 
+lemma evalYulStep_cont_extend_fail :
+  assumes Hstep : "evalYulStep D \<lparr>result = r, cont = h#t\<rparr> = 
+                   ErrorResult msg bad"
+  shows "\<exists>  bad' . evalYulStep D \<lparr> result = r, cont = [h] \<rparr> =
+           ErrorResult msg bad'" 
+proof(cases "r_mode r")
+  case Regular
+  then show ?thesis
+  proof(cases h)
+    case (EnterStatement st)
+    then show ?thesis using assms Regular
+      by(auto simp add: updateResult_def split: YulResult.splits option.splits)
+  next
+    case (ExitStatement st L F)
+    then show ?thesis using assms Regular
+      by(auto simp add: updateResult_def split: YulResult.splits option.splits)
+  next
+    case (EnterFunctionCall name fsig)
+    then show ?thesis using assms Regular
+      by(auto simp add: updateResult_def split: YulResult.splits option.splits)
+  next
+    case (ExitFunctionCall name vals_old local_old funs_old fsig)
+    then show ?thesis using assms Regular
+      by(auto simp add: updateResult_def split: YulResult.splits option.splits)
+  next
+    case (Expression e)
+    then show ?thesis using assms Regular
+      by(auto simp add: updateResult_def split: YulResult.splits option.splits)
+  qed
+next
+  case Break
+  then show ?thesis  using Hstep
+    by(cases h; auto split: YulStatement.splits)
+  next
+  case Continue
+  then show ?thesis  using Hstep
+    by(cases h; auto split: YulStatement.splits)
+next
+  case Leave
+  then show ?thesis  using Hstep
+    by(cases h; auto split: YulStatement.splits)
+qed
+
+
+lemma evalYul'_pres_fail :
+  assumes H : "evalYul' D input n = ErrorResult msg res"
+  assumes Leq : "n \<le> n'"
+  shows "evalYul' D input n' = ErrorResult msg res" using assms
+proof(induction n arbitrary: D input n' msg res)
+  case 0
+  then show ?case by auto
+next
+  case (Suc n)
+  show ?case
+  proof(cases "cont input")
+    case Nil
+    then show ?thesis using Suc.prems
+      by(auto)
+  next
+    case (Cons ch ct)
+    
+    show ?thesis
+    proof(cases "evalYulStep D input")
+      case (ErrorResult msg' res')
+      then show ?thesis using Suc.prems by(auto)
+    next
+      case (YulResult res')
+  
+      then have Eval' : "evalYul' D res' n = ErrorResult msg res"
+        using Suc.prems Cons by auto
+  
+      show ?thesis using Suc.prems
+      proof(cases "n' - Suc n")
+        case Zero' : 0
+        then show ?thesis using Suc.prems YulResult by auto
+      next
+        case Suc' : (Suc diff1)
+
+        hence Leq : "n \<le> n' - 1" using Suc.prems by auto
+
+        have NZ : "1 + (n' - 1) = n'" using Suc by auto
+  
+        have Penult :
+          "evalYul' D res' (n' - 1) = ErrorResult msg res" 
+          using Suc.IH[OF Eval' Leq] by auto
+  
+        have FirstStep :
+          "evalYul' D input 1 = YulResult res'"
+          using YulResult
+          by(auto split:YulMode.splits)
+  
+        have Conc' : "evalYul' D input (1 + (n' - 1)) = ErrorResult msg res"
+          using evalYul'_steps[OF FirstStep Penult] by auto
+  
+        then show ?thesis unfolding NZ by auto
+      qed
+    qed
+  qed
+qed
+
+lemma evalYul'_pres_succeed :
+  assumes H : "evalYul' D input n = YulResult res"
+  assumes Hcont : "cont res = []"
+  assumes Leq : "n \<le> n'"
+  shows "evalYul' D input n' = YulResult res" using assms
+proof(induction n arbitrary: D input n' res)
+  case 0
+  then show ?case by auto
+next
+  case (Suc n)
+
+  show ?case
+  proof(cases "cont input")
+    case Nil
+    then show ?thesis using Suc.prems
+      by(auto)
+  next
+    case (Cons ch ct)
+    
+    show ?thesis
+    proof(cases "evalYulStep D input")
+      case (ErrorResult msg' res')
+      then show ?thesis using Suc.prems Cons by(auto)
+    next
+      case (YulResult res1)
+  
+      then have Eval' : "evalYul' D res1 n = YulResult res"
+        using Suc.prems Cons by auto
+  
+      show ?thesis
+      proof(cases "n' - Suc n")
+        case Zero' : 0
+        then show ?thesis using Suc.prems YulResult by auto
+      next
+        case Suc' : (Suc diff1)
+
+        hence Leq : "n \<le> n' - 1" using Suc.prems by auto
+
+        have NZ : "1 + (n' - 1) = n'" using Suc by auto
+  
+        have Penult :
+          "evalYul' D res1 (n' - 1) = YulResult res" 
+          using Suc.IH[OF Eval' Suc.prems(2) Leq] by auto
+  
+        have FirstStep :
+          "evalYul' D input 1 = YulResult res1"
+          using YulResult
+          by(auto split:YulMode.splits)
+  
+        have Conc' : "evalYul' D input (1 + (n' - 1)) = YulResult res"
+          using evalYul'_steps[OF FirstStep Penult] by auto
+  
+        then show ?thesis unfolding NZ by auto
+      qed
+    qed
+  qed
+qed
+  
+(* ok, so now for local reasoning.
+   there is a complication here, which is that it would be better to show that
+   n1 is exactly the right number of steps to first reach []
+*)
+
+lemma evalYulStep_minsteps :
+  assumes H : "evalYul' D \<lparr> result = r, cont = c \<rparr> n = YulResult \<lparr> result = rfin, cont = []\<rparr>"
+  shows "\<exists> n' . n' \<le> n \<and> 
+                evalYul' D \<lparr> result = r, cont = c \<rparr> n' = YulResult \<lparr> result = rfin, cont = [] \<rparr> \<and>
+                (\<forall> x . x < n' \<longrightarrow>
+                  (\<exists> r' ch ct .
+                    evalYul' D \<lparr> result = r, cont = c \<rparr> x = 
+                    YulResult \<lparr> result = r', cont = ch#ct \<rparr> ))" using H
+proof(induction n arbitrary: r c rfin)
+  case 0
+  then show ?case by(auto)
+next
+  case (Suc n)
+  show ?case 
+  proof(cases "evalYul' D \<lparr>result = r, cont = c\<rparr> n")
+    case (ErrorResult x21 x22)
+    show ?thesis using evalYul'_pres_fail[OF ErrorResult, of "Suc n"] Suc.prems by auto
+  next
+    case (YulResult res1)
+
+    obtain r1 c1 where Res1 : "res1 = \<lparr> result = r1, cont = c1 \<rparr>" by(cases res1; auto)
+
+    show ?thesis
+    proof(cases c1)
+      case Nil
+
+      have YR' : "evalYul' D \<lparr>result = r, cont = c\<rparr> n = YulResult \<lparr> result = r1, cont = [] \<rparr>"
+        using YulResult Nil Res1 by simp
+
+      obtain n' where Leq : "n' \<le> n"
+                and Conc'1 : 
+                    "evalYul' D \<lparr>result = r, cont = c\<rparr> n' = YulResult \<lparr>result = r1, cont = []\<rparr>"
+                and Conc'2 :
+                        "(\<forall>x<n'. \<exists>r' ch ct. evalYul' D \<lparr>result = r, cont = c\<rparr> x = 
+                              YulResult \<lparr>result = r', cont = ch # ct\<rparr>)"
+        using Suc.IH[OF YR'] by auto
+
+      have Leq' : "n' \<le> Suc n" using Leq by auto
+
+      have R1Eq : "r1 = rfin"
+        using evalYul'_pres_succeed[OF Conc'1 _ Leq'] Suc.prems by auto
+
+      show ?thesis using Leq' Conc'1 Conc'2 unfolding R1Eq by blast
+    next
+      case (Cons c1h c1t)
+
+      have YR' : "evalYul' D \<lparr>result = r, cont = c\<rparr> n = YulResult \<lparr> result = r1, cont = c1h#c1t \<rparr>"
+        using YulResult Cons Res1 by simp
+
+      (* In this case Suc n is itself the minimal number of steps. *)
+      have Conc'2 :
+        "\<And> x . x < Suc n \<Longrightarrow> \<exists>r' ch ct. evalYul' D \<lparr>result = r, cont = c\<rparr> x = 
+                    YulResult \<lparr>result = r', cont = ch # ct\<rparr>"
+      proof-
+        fix x
+        assume Hx : "x < Suc n"
+
+        hence Xleq : "x \<le> n" by auto
+
+        show "\<exists>r' ch ct. evalYul' D \<lparr>result = r, cont = c\<rparr> x = 
+                YulResult \<lparr>result = r', cont = ch # ct\<rparr>"
+        proof(cases "evalYul' D \<lparr>result = r, cont = c\<rparr> x")
+          case ErrorResult' : (ErrorResult x21 x22)
+          show ?thesis using evalYul'_pres_fail[OF ErrorResult', of "Suc n"] Suc.prems Hx
+            by auto
+        next
+          case YulResult' : (YulResult resx)
+
+          show ?thesis
+          proof(cases "cont resx")
+            case Nil' : Nil
+
+            have False using evalYul'_pres_succeed[OF YulResult' Nil' Xleq ] YR' Nil'
+              by(cases resx; auto)
+
+            then show ?thesis by auto
+          next
+            case (Cons rxh rxt)
+            then show ?thesis using YulResult'
+              by(cases resx; auto)
+          qed
+        qed
+      qed
+
+      show ?thesis using Suc.prems Conc'2 by blast
+    qed
+  qed
+qed
+
+
+(* if we're not done evaluating, what's in the tail doesn't matter
+   *)
+lemma evalYul'_cont_extend :
+  assumes H : "evalYul' D \<lparr> result = ri, cont = ci \<rparr> n = YulResult \<lparr> result = rf, cont = cf\<rparr>"
+  assumes Hcont : "cf = cfh#cft"
+  shows "evalYul' D \<lparr> result = ri, cont = ci @ post \<rparr> n = 
+                      YulResult \<lparr> result = rf, cont = cf @ post \<rparr>" using assms
+proof(induction n arbitrary: ri ci rf cf post )
+  case 0
+  then show ?case 
+    by(auto)
+next
+  case (Suc n)
+  then show ?case
+
+  proof(cases "evalYulStep D \<lparr> result = ri, cont = ci \<rparr>")
+    case (ErrorResult msg res1)
+
+    then show ?thesis 
+    proof(cases "ci")
+      case Nil
+      then show ?thesis using Suc.prems by auto
+    next
+      case (Cons cih cit)
+      then show ?thesis 
+        using Suc.prems ErrorResult by auto
+    qed
+  next
+    case (YulResult res1)
+
+    obtain r1 c1 where Res1 : "res1 = \<lparr> result = r1, cont = c1 \<rparr>" by(cases res1; auto)
+
+    show ?thesis
+    proof(cases c1)
+      case Nil
+
+      have YR' : "evalYul' D \<lparr> result = ri, cont = ci \<rparr> 1 = YulResult \<lparr> result = r1, cont = [] \<rparr>"
+        using YulResult Nil Res1 
+        by(cases "ci"; simp split:YulMode.splits)
+
+      have False using evalYul'_pres_succeed[OF YR', of "Suc n"] Suc.prems by auto
+
+      thus ?thesis by auto
+    next
+      case (Cons c1h c1t)
+
+      have YR' : "evalYul' D \<lparr> result = ri, cont = ci \<rparr> 1 = 
+                  YulResult \<lparr> result = r1, cont = c1h#c1t \<rparr>"
+        using YulResult Cons Res1
+        by(cases "ci"; simp split:YulMode.splits)
+
+      show ?thesis
+      proof(cases "evalYul' D \<lparr> result = r1, cont = c1h#c1t \<rparr> n")
+        case ErrorResult' : (ErrorResult msg2 res2)
+
+        have False using evalYul'_steps[OF YR' ErrorResult'] Suc.prems by auto
+
+        thus ?thesis by auto
+      next
+        case YulResult' : (YulResult res2)
+
+        have Res2 : "res2 = \<lparr> result = rf, cont = cf\<rparr>"
+          using evalYul'_steps[OF YR' YulResult'] Suc.prems by auto
+
+        have Rest : "evalYul' D \<lparr> result = r1, cont = c1h#c1t \<rparr> n = 
+                     YulResult \<lparr> result = rf, cont = cf\<rparr>"
+          using YulResult' unfolding Res2 by auto
+
+        have IHspec: "evalYul' D \<lparr>result = r1, cont = c1h#c1t @ post\<rparr> n =
+                       YulResult\<lparr> result = result res2, cont = cont res2 @ post \<rparr>"
+          using Suc.IH[OF Rest] Suc.prems Res2
+          by auto
+
+        show ?thesis
+        proof(cases "ci")
+          case Nil' : Nil
+          then show ?thesis using Suc.prems by auto
+        next
+          case Cons' : (Cons cih cit)
+          obtain res1_pre where 
+            Res1_pre : "c1h#c1t = res1_pre @ cit" and
+            Res1_pre_eval : "evalYulStep D \<lparr>result = ri, cont = [cih]\<rparr> = 
+                             YulResult \<lparr>result = r1, cont = res1_pre\<rparr>"
+            using evalYulStep_cont_extend[of D "ri" "cih" "cit" r1 c1] YulResult 
+                  Cons' Res1 Cons
+            by(auto)
+
+          show ?thesis
+          proof(cases "evalYulStep D \<lparr> result = ri, cont = cih#cit@post \<rparr>")
+            case ErrorResult'' : (ErrorResult msg3 bad3)
+
+            have False using evalYulStep_cont_extend_fail[OF ErrorResult''] Res1_pre_eval
+              by auto
+
+            then show ?thesis by auto
+          next
+            case YulResult''' : (YulResult res3)
+
+            obtain r3 c3 where Res3 : "res3 = \<lparr> result = r3, cont = c3 \<rparr>" by(cases res3; auto)
+
+            obtain res3_pre where
+              Res3_pre : "c3 = res3_pre @ cit@post" and
+              Res3_pre_eval : "evalYulStep D \<lparr>result = ri, cont = [cih]\<rparr> = 
+                                YulResult \<lparr>result = r3, cont = res3_pre\<rparr>"
+              using evalYulStep_cont_extend[of D "ri" "cih" "cit@post" r3 c3] 
+                  YulResult''' Res3
+                  Cons' Res3 Cons
+              by auto
+
+            have R1_R3 : "r1 = r3"
+              using Res3_pre_eval Res1_pre_eval by auto
+
+            have R1pre_R3pre : "res1_pre = res3_pre"
+              using Res3_pre_eval Res1_pre_eval by auto
+
+            have YR''' : "evalYul' D \<lparr> result = ri, cont = cih#cit@post \<rparr> 1 = 
+                        YulResult \<lparr> result = r1, cont = c1h#c1t@post \<rparr>"
+              using YulResult''' Cons Res1 Res3 R1_R3 R1pre_R3pre 
+                    Res1_pre Res1_pre_eval
+                    Res3_pre Res3_pre_eval
+              by(simp split:YulMode.splits)
+
+
+            show ?thesis
+              using evalYul'_steps[OF YR''' IHspec] Res2 Cons'
+              by(auto)
+          qed
+        qed
+      qed
+    qed
+  qed
+qed
+
+(* generalization: assume a potentially nonempty residual continuation after running first command? *)
+
+lemma evalYul'_seq :
+  assumes H1 : "evalYul' D \<lparr>result = r1, cont = c1\<rparr> n1 = 
+               YulResult \<lparr>result = r2, cont = residue\<rparr>"
+  assumes H2 : "evalYul' D \<lparr>result = r2, cont = residue @ c2 \<rparr> n2 = YulResult \<lparr> result = r3, cont = [] \<rparr>"
+  shows "evalYul' D \<lparr> result = r1, cont = c1 @ c2\<rparr> (n1 + n2) = YulResult \<lparr> result = r3, cont = [] \<rparr>" using assms
+proof(induction n1 arbitrary: r1 c1 r2 residue c2 n2 r3)
+  case 0
+  then show ?case
+    by auto
+next
+  case (Suc n1)
+
+  show ?case
+  proof(cases c1)
+    case Nil
+
+    then have AlreadyDone : 
+      "evalYul' D \<lparr>result = r1, cont = c1\<rparr> 0 = YulResult \<lparr>result = r1, cont = c1\<rparr>"
+      by(auto)
+
+    have R2 : "r1 = r2" and Residue : "residue = []"
+      using evalYul'_pres_succeed[OF AlreadyDone, of "Suc n1"] Suc.prems(1) Nil
+      by auto
+
+    have Conc' : "evalYul' D \<lparr>result = r2, cont = c2\<rparr> n2 = YulResult \<lparr>result = r3, cont = []\<rparr>"
+      using Suc.prems(2) unfolding R2 Residue Nil by auto
+
+    show ?thesis using evalYul'_pres_succeed[OF Conc', of "Suc n1 + n2"]
+      unfolding R2 Residue Nil by auto
+  next
+    case (Cons c1h c1t)
+
+    show ?thesis
+    proof(cases "evalYulStep D \<lparr>result = r1, cont = c1\<rparr>")
+      case (ErrorResult msg rbad)
+  
+      then have False using Suc Cons
+        by(cases c1; simp del:evalYulStep.simps)
+
+      thus ?thesis by auto
+    next
+      case (YulResult res1')
+
+      obtain r1' c1' where Res1' : "res1' = \<lparr> result = r1', cont = c1' \<rparr>"
+        by(cases res1'; auto)
+
+      have Eval' : "evalYul' D \<lparr>result = r1', cont = c1'\<rparr> n1 =
+                    YulResult \<lparr>result = r2, cont = residue\<rparr>"
+        using Res1' Suc.prems YulResult Cons by auto
+
+      have IHspec : "evalYul' D \<lparr>result = r1', cont = c1' @ c2\<rparr> (n1 + n2) =
+              YulResult \<lparr>result = r3, cont = []\<rparr>"
+        using Suc.IH[OF Eval'] (* Suc.prems(2) *) Suc.prems(2)
+        by auto
+
+      (* need a "first step" lemma *)
+
+      obtain c1'_new where
+        C1'_new_step : "evalYulStep D \<lparr>result = r1, cont = [c1h] \<rparr> = 
+                        YulResult \<lparr>result = r1', cont = c1'_new\<rparr>" and
+        C1'_new_pre : "c1' = c1'_new @ c1t"
+        using evalYulStep_cont_extend[of D r1 c1h c1t r1' c1'] YulResult Cons Res1'
+        by auto
+
+      have FirstStep' : "evalYul' D \<lparr>result = r1, cont = c1h#c1t \<rparr> 1 = YulResult \<lparr> result = r1', cont = c1' \<rparr>"
+        using Res1' YulResult Cons
+        by(auto)
+
+      show ?thesis
+      proof(cases "evalYulStep D \<lparr>result = r1, cont = c1 @ c2\<rparr>")
+        case ErrorResult' : (ErrorResult msg rbad)
+
+        hence ER' : "evalYulStep D \<lparr>result = r1, cont = c1h# (c1t @ c2)\<rparr> = ErrorResult msg rbad" 
+          using Cons by auto
+
+        have False using evalYulStep_cont_extend_fail[OF ER'] C1'_new_step by auto
+
+        thus ?thesis by auto
+      next
+        case YulResult' : (YulResult res1'')
+
+        obtain r1'' c1'' where Res1'' : "res1'' = \<lparr> result = r1'', cont = c1'' \<rparr>"
+          by(cases res1''; auto)
+
+        have YR' : "evalYulStep D \<lparr>result = r1, cont = c1h # (c1t @ c2)\<rparr> =
+                    YulResult \<lparr> result = r1'', cont = c1'' \<rparr>"
+          using YulResult' unfolding Res1'' Cons by auto
+
+        have C1'' : "c1'' = c1'_new @ (c1t @ c2)" and R1'' : "r1'' = r1'"
+          using evalYulStep_cont_extend[OF YR'] C1'_new_step C1'_new_pre
+          by auto
+
+        hence C1''_C1' : "c1'' = c1' @ c2" using C1'_new_pre
+          by simp
+
+        have FirstStep : "evalYul' D \<lparr>result = r1, cont = c1 @ c2\<rparr> 1 = 
+                          YulResult \<lparr> result = r1', cont = c1' @ c2 \<rparr> "
+          using YR' unfolding Cons C1''_C1' R1''
+        by(auto)
+
+      show ?thesis using evalYul'_steps[OF FirstStep IHspec] by auto
+    qed
+  qed
+qed
+
+
+(* evalYul' D \<lparr>result = r1, cont = c1 @ c2\<rparr> = YulResult \<lparr>result = r1', cont = c1' @ c2\<rparr>  *)
+(*
+      proof(cases residue)
+      case Nil' : Nil
+        then show ?thesis using evalYul'_steps
+      next
+        case (Cons resdh resdt)
+        then show ?thesis sorry
+      qed
+
+      show ?thesis using evalYul'_steps
+*)
+(* idea: apply continuation-decomposition here to show that we get what we expect after the first step *)
+(* may need a lemma saying what happens when we add a suffix.
+probably this will require a case analysis on residue...?
+ *)
+  
+(*
+  show ?case
+  proof(cases c1)
+    case Nil
+    show ?thesis
+      using Suc
+
+
+    proof(cases c2)
+      case Nil' : Nil
+      then show ?thesis using Suc Nil by(cases n2; auto)
+    next
+      case (Cons c2h c2t)
+
+(*
+      obtain r2' where R2' : "evalYulStep D \<lparr>result = r2, cont = c2h # c2t\<rparr> = YulResult r2'"
+        using Suc.prems Nil Cons
+        by(cases n2; cases "evalYulStep D \<lparr>result = r2, cont = c2h # c2t\<rparr>"; 
+                           auto simp del: evalYulStep.simps)
+*)
+      show ?thesis
+      proof(cases "evalYul' D \<lparr>result = r1, cont = c1\<rparr> n1")
+        case (ErrorResult x21 x22)
+
+        have False using evalYul'_pres_fail[OF ErrorResult, of "Suc n1"] Suc.prems(1)
+          by auto
+
+        then show ?thesis by auto
+      next
+        case (YulResult res1')
+
+        obtain r1' c1' where Res1' : "res1' = \<lparr> result = r1', cont = c1' \<rparr>"
+          by(cases res1'; auto)
+
+        have YR' : "evalYul' D \<lparr>result = r1, cont = c1\<rparr> n1 = YulResult \<lparr> result = r1', cont = c1' \<rparr>"
+          using YulResult unfolding Res1' by auto
+
+        show ?thesis using Suc.IH YR'
+        
+      qed
+  next
+    case (Cons a list)
+    then show ?thesis sorry
+  qed
+
+        apply(auto simp del: evalYulStep.simps)
+
+
+  proof(cases n1)
+    case Zero' : 0
+    show ?thesis
+    proof(cases n2)
+      case Zero'' : 0
+      then show ?thesis 
+        using Suc Zero' by(auto)
+    next
+      case Suc'' : (Suc nat)
+      then show ?thesis using Suc Zero'
+        apply(auto simp del: evalYulStep.simps)
+    qed
+
+    then show ?thesis using Suc apply(auto simp del: evalYulStep.simps)
+  next
+    case (Suc nat)
+    then show ?thesis sorry
+  qed
+
+    apply(auto simp del: evalYulStep.simps)
+
+
+
+  proof(cases "evalYulStep D \<lparr>result = r2', cont = xh # xt\<rparr>")
+    case (YulResult x1)
+    show ?thesis
+      using YulResult 0 apply(auto simp del: evalYulStep.simps)
+
+    proof(cases "evalYulStep D \<lparr>result = r2', cont = xh # xt @ c2\<rparr> ")
+      case YulResult' : (YulResult x1')
+      then show ?thesis using YulResult 0 apply(auto simp del: evalYulStep.simps)
+    next
+      case (ErrorResult x21 x22)
+      then show ?thesis sorry
+    qed
+    then show ?thesis using 0 apply(auto simp del: evalYulStep.simps)
+  next
+    case (ErrorResult x21 x22)
+    then show ?thesis sorry
+  qed
+    
+    apply(auto simp del: evalYulStep.simps)
+next
+  case (Suc n1)
+  show ?case
+  proof(cases c1)
+    case Nil
+    then show ?thesis using Suc.prems(1) Suc.prems(2) apply(cases c2; auto)
+      apply(cases "r_mode r2"; auto) 
+  next
+    case (Cons a list)
+    then show ?thesis sorry
+  qed
+
+  show ?case using Suc.prems(1) Suc.prems(2)
+    apply(auto simp del: evalYulStep.simps)
+    apply(cases c1; auto)
+    
+  next
+    case Suc' : (Suc n1')
+    then show ?thesis sorry
+  qed
+
+    apply(auto)
+qed
+*)
 (* reasoning about Seq. idea:
    - EnterStatement (spre  @ spost) becomes
    - (map statement spre) @ (map statement spost)   
